examples/unit-tests/testset.fst
@@ -1,0 +1,28 @@
+module TestSet
+assume type elt
+assume logic val A : elt
+assume logic val B : elt
+assume logic val C : elt
+assume AB_distinct: A=!=B
+
+val should_succeed: unit -> Tot unit
+let should_succeed u =
+  assert (InSet B (Union (Singleton A) (Singleton B)));
+  assert (InSet A (Union (Singleton A) (Singleton B)));
+  assert (Subset (Singleton A) (Union (Singleton A) (Singleton B)));
+  assert (Subset (Singleton B) (Union (Singleton A) (Singleton B)));
+  assert (SetEqual (Union (Singleton A) (Singleton B))
+                   (Union (Singleton B) (Singleton A)))
+
+val should_fail1: unit -> Tot unit
+let should_fail1 u =
+  assert (InSet B (Singleton A))
+
+val should_fail2: unit -> Tot unit
+let should_fail2 u = 
+  assert (Subset (Union (Singleton A) (Singleton B)) (Singleton A))
+
+val should_fail3: unit -> Tot unit
+let should_fail3 u =
+  assert (InSet C (Union (Singleton A) (Singleton B)))
+            
